theories/typing/shr_bor.v
@@ -1,3 +1,4 @@
+From iris.base_logic Require Import big_op.
 From iris.proofmode Require Import tactics.
 From lrust.lifetime Require Import frac_borrow.
 From lrust.typing Require Export type.
@@ -14,7 +15,7 @@ Section shr_bor.
     iIntros (κ ty tid vl) "H". iDestruct "H" as (l) "[% _]". by subst.
   Qed.
 
-  Global Instance subtype_shr_mono E L :
+  Global Instance subtype_shr_bor_mono E L :
     Proper (flip (incl E L) ==> subtype E L ==> subtype E L) shr_bor.
   Proof.
     intros κ1 κ2 Hκ ty1 ty2 Hty. split.
@@ -25,17 +26,18 @@ Section shr_bor.
       iSplit. done. by iApply (ty2.(ty_shr_mono) with "LFT Hκ"); last iApply "Hty".
     - iIntros (qE qL) "#LFT HE HL *". iDestruct (Hκ with "HE HL") as "#Hκ".
       iDestruct (subtype_shr _ _ _ _ Hty with "LFT HE HL") as "#Hst".
-      iIntros "{HE HL}!#*H". iDestruct "H" as (vl) "#[Hfrac Hty]".
-      iExists vl. iFrame "#". iNext.
-      iDestruct "Hty" as (l0) "(% & Hty)". subst. iExists _. iSplit. done.
-      by iApply (ty_shr_mono with "LFT Hκ"); last iApply "Hst".
+      iIntros "{HE HL}!#*H". iDestruct "H" as (vl) "#[Hfrac [Hty|H†]]".
+      + iExists vl. iFrame "#". iLeft. iNext. simpl.
+        iDestruct "Hty" as (l0) "(% & Hty)". subst. iExists _. iSplit. done.
+          by iApply (ty_shr_mono with "LFT Hκ"); last iApply "Hst".
+      + simpl. eauto.
   Qed.
-  Global Instance subtype_shr_mono' E L :
+  Global Instance subtype_shr_bor_mono' E L :
     Proper (incl E L ==> flip (subtype E L) ==> flip (subtype E L)) shr_bor.
-  Proof. intros ??????. by apply subtype_shr_mono. Qed.
-  Global Instance subtype_shr_proper E L κ :
+  Proof. intros ??????. by apply subtype_shr_bor_mono. Qed.
+  Global Instance subtype_shr_bor_proper E L κ :
     Proper (eqtype E L ==> eqtype E L) (shr_bor κ).
-  Proof. intros ??[]. by split; apply subtype_shr_mono. Qed.
+  Proof. intros ??[]. by split; apply subtype_shr_bor_mono. Qed.
 End shr_bor.
 
 Notation "&shr{ κ } ty" := (shr_bor κ ty)
@@ -44,14 +46,14 @@ Notation "&shr{ κ } ty" := (shr_bor κ ty)
 Section typing.
   Context `{typeG Σ}.
 
-  Lemma perm_incl_share q ν κ ty :
-    ν ◁ &uniq{κ} ty ∗ q.[κ] ⇒ ν ◁ &shr{κ} ty ∗ q.[κ].
+  Lemma tctx_incl_share E L p κ ty :
+    tctx_incl E L [TCtx_holds p (&uniq{κ}ty)] [TCtx_holds p (&shr{κ}ty)].
   Proof.
-    iIntros (tid) "#LFT [Huniq [Htok $]]". unfold has_type.
-    destruct (eval_expr ν); last by iDestruct "Huniq" as "[]".
+    iIntros (??) "#LFT _ _ !# * Huniq". rewrite /tctx_interp !big_sepL_singleton /=.
+    iDestruct "Huniq" as (v) "[% Huniq]". iExists _. iFrame "%".
     iDestruct "Huniq" as (l P) "[[% #HPiff] HP]".
     iMod (bor_iff with "LFT [] HP") as "H↦". set_solver. by eauto.
-    iMod (ty.(ty_share) _ lrustN with "LFT H↦ Htok") as "[Hown $]"; [solve_ndisj|done|].
+    iMod (ty.(ty_share) _ lrustN with "LFT H↦") as "Hown"; [solve_ndisj|done|].
     iIntros "!>/=". eauto.
   Qed.
 
@@ -93,14 +95,16 @@ Section typing.
     iIntros (tid) "!#(#HEAP & #LFT & (H◁ & #H⊑ & Htok) & $)". wp_bind ν.
     iApply (has_type_wp with "H◁"). iIntros (v) "Hνv H◁!>". iDestruct "Hνv" as %Hνv.
     rewrite has_type_value. iDestruct "H◁" as (l) "[Heq #H↦]". iDestruct "Heq" as %[=->].
-    iMod (lft_incl_acc with "H⊑ Htok") as (q'') "[[Htok1 Htok2] Hclose]". done.
+    iMod (lft_incl_acc with "H⊑ Htok") as (q'') "[Htok Hclose]". done.
     iDestruct "H↦" as (vl) "[H↦b #Hown]".
-    iMod (frac_bor_acc with "LFT H↦b Htok1") as (q''') "[>H↦ Hclose']". done.
-    iApply (wp_fupd_step _ (⊤∖↑lrustN) with "[Hown Htok2]"); try done.
-    - iApply ("Hown" with "* [%] Htok2"). set_solver.
-    - wp_read. iIntros "!>[Hshr ?]". iFrame "H⊑".
-      iSplitL "Hshr"; first by iExists _; auto. iApply ("Hclose" with ">").
-      iFrame. iApply "Hclose'". auto.
+    iMod (frac_bor_acc with "LFT H↦b Htok") as (q''') "[>H↦ Hclose']". done.
+    iApply (wp_fupd_step _ (⊤∖↑lrustN∖↑lftN) with "[Hown]"); try done.
+    - iApply ("Hown" with "* [%]"). set_solver.
+    - wp_read. iIntros "!>[Hshr|#H†]{$H⊑}".
+      + iSplitL "Hshr"; first by iExists _; auto. iApply ("Hclose" with ">").
+        iFrame. iApply "Hclose'". auto.
+      + iMod ("Hclose'" with "[H↦]"). by auto.
+        by iDestruct (lft_tok_dead with "[-] H†") as "[]".
   Qed.
 
   Lemma typed_deref_shr_bor_bor ty ν κ κ' κ'' q:
@@ -112,16 +116,17 @@ Section typing.
     iApply (has_type_wp with "H◁"). iIntros (v) "Hνv H◁!>". iDestruct "Hνv" as %Hνv.
     rewrite has_type_value. iDestruct "H◁" as (l) "[Heq Hshr]".
     iDestruct "Heq" as %[=->]. iDestruct "Hshr" as (l') "[H↦ Hown]".
-    iMod (lft_incl_acc with "H⊑1 Htok") as (q') "[[Htok1 Htok2] Hclose]". done.
-    iMod (frac_bor_acc with "LFT H↦ Htok1") as (q'') "[>H↦ Hclose']". done.
+    iMod (lft_incl_acc with "H⊑1 Htok") as (q') "[Htok Hclose]". done.
+    iMod (frac_bor_acc with "LFT H↦ Htok") as (q'') "[>H↦ Hclose']". done.
     iAssert (κ' ⊑ κ'' ∪ κ')%I as "#H⊑3".
     { iApply (lft_incl_glb with "H⊑2 []"). iApply lft_incl_refl. }
-    iMod (lft_incl_acc with "H⊑3 Htok2") as (q''') "[Htok Hclose'']". done.
-    iApply (wp_fupd_step _ (_∖_) with "[Hown Htok]"); try done.
-    - iApply ("Hown" with "* [%] Htok"). set_solver.
-    - wp_read. iIntros "!>[Hshr Htok]". iFrame "H⊑1". iSplitL "Hshr".
-      + iExists _. iSplitR. done. by iApply (ty_shr_mono with "LFT H⊑3 Hshr").
-      + iApply ("Hclose" with ">"). iMod ("Hclose'" with "[$H↦]") as "$".
-        by iMod ("Hclose''" with "Htok") as "$".
+    iApply (wp_fupd_step _ (_∖_) with "[Hown]"); try done.
+    - iApply ("Hown" with "* [%]"). set_solver.
+    - wp_read. iIntros "!>[#Hshr|#H†]{$H⊑1}".
+      + iSplitR.
+        * iExists _. iSplitR. done. by iApply (ty_shr_mono with "LFT H⊑3 Hshr").
+        * iApply ("Hclose" with ">"). iApply ("Hclose'" with "[$H↦]").
+      + iMod ("Hclose'" with "[H↦]"). by auto.
+        by iDestruct (lft_tok_dead with "[-] H†") as "[]".
   Qed.
 End typing.
